Recast clos's remove optimisation
1. It has to check that the removed expressions are pure
2. It doesn't have to remove expressions in blocks, but can selectively
   remove single expressions within binding blocks (the es of Let es x)

compiler/backend/clos_removeScript.sml
@@ -8,10 +8,64 @@ open preamble db_varsTheory closLangTheory;
 
 val _ = new_theory"clos_remove";
 
+val pure_op_def = Define `
+  pure_op op ⇔
+    case op of
+      FFI _ => F
+    | SetGlobal _ => F
+    | AllocGlobal => F
+    | RefByte => F
+    | RefArray => F
+    | UpdateByte => F
+    | Equal => F
+    | Ref => F
+    | Update => F
+    | _ => T
+`;
+
+(* pure e means e can neither raise an exception nor side-effect the state *)
+val pure_def = tDefine "pure" `
+  (pure (Var _) ⇔ T)
+    ∧
+  (pure (If e1 e2 e3) ⇔ pure e1 ∧ pure e2 ∧ pure e3)
+    ∧
+  (pure (Let es e2) ⇔ EVERY pure es ∧ pure e2)
+    ∧
+  (pure (Raise _) ⇔ F)
+    ∧
+  (pure (Handle e1 _) ⇔ pure e1)
+    ∧
+  (pure (Tick _) ⇔ F)
+    ∧
+  (pure (Call _ _) ⇔ F)
+    ∧
+  (pure (App _ _ _) ⇔ F)
+    ∧
+  (pure (Fn _ _ _ _) ⇔ T)
+    ∧
+  (pure (Letrec _ _ fns x) ⇔ EVERY (λ(n,e). pure e) fns ∧ pure x)
+    ∧
+  (pure (Op opn es) ⇔ EVERY pure es ∧ pure_op opn)
+` (WF_REL_TAC `measure exp_size` >> simp[] >> rpt conj_tac >> rpt gen_tac >>
+   (Induct_on `es` ORELSE Induct_on `fns`) >> dsimp[exp_size_def] >>
+   rpt strip_tac >> res_tac >> simp[])
+
 val no_overlap_def = Define `
   (no_overlap 0 l <=> T) /\
   (no_overlap (SUC n) l <=>
      if has_var n l then F else no_overlap n l)`
+
+val MAPi_def = Define`
+  MAPi f l = REVERSE (SND (FOLDL (λ(n,a) e. (n + 1n, f n e :: a)) (0,[]) l))
+`;
+val MAPi_CONG = store_thm(
+  "MAPi_CONG[defncong]",
+  ``∀(l1:α list) l2 (f1:num -> α -> β) f2.
+      (l1 = l2) ∧ (∀n e. MEM e l2 ⇒ f1 n e = f2 n e) ⇒
+      MAPi f1 l1 = MAPi f2 l2``,
+  simp[MAPi_def] >> SPEC_TAC(``0n``, ``i:num``) >>
+  SPEC_TAC(``[] : β list``, ``a : β list``) >>
+  Induct_on `l2` >> dsimp[]);
 
 val const_0_def = Define `
   const_0 = Op (Const 0) []`;
@@ -29,13 +83,17 @@ val remove_def = tDefine "remove" `
      let (c3,l3) = remove [x3] in
        ([If (HD c1) (HD c2) (HD c3)],mk_Union l1 (mk_Union l2 l3))) /\
   (remove [Let xs x2] =
-     let n = LENGTH xs in
      let (c2,l2) = remove [x2] in
-       if no_overlap n l2 then
-         ([Let (REPLICATE n const_0) (HD c2)], Shift n l2)
-       else
-         let (c1,l1) = remove xs in
-           ([Let c1 (HD c2)],mk_Union l1 (Shift n l2))) /\
+     let xls =
+       MAPi (λi e. if has_var i l2 ∨ ¬pure e then
+                     let (c,l) = remove [e] in
+                       (HD c, l)
+                   else (const_0, Empty)) xs in
+     let (xs', frees) = FOLDR (λ(x,l) (ts,frees). x::ts, mk_Union l frees)
+                              ([], Shift (LENGTH xs) l2)
+                              xls
+     in
+       ([Let xs' (HD c2)], frees)) /\
   (remove [Raise x1] =
      let (c1,l1) = remove [x1] in
        ([Raise (HD c1)],l1)) /\
@@ -55,15 +113,19 @@ val remove_def = tDefine "remove" `
   (remove [Letrec loc vs_opt fns x1] =
      let m = LENGTH fns in
      let (c2,l2) = remove [x1] in
-       if no_overlap m l2 then
-         ([Let (REPLICATE m const_0) (HD c2)], Shift m l2)
-       else
-         let res = MAP (\(n,x). let (c,l) = remove [x] in
-                                  ((n,HD c),Shift (n + m) l)) fns in
-         let c1 = MAP FST res in
-         let l1 = list_mk_Union (MAP SND res) in
-           ([Letrec loc vs_opt c1 (HD c2)],
-            mk_Union l1 (Shift (LENGTH fns) l2))) /\
+     let xls =
+       MAPi (λi (n,x).
+                if has_var i l2 ∨ ¬pure x then
+                  let (c,l) = remove [x] in
+                    ((n, HD c), Shift (n + m) l)
+                else
+                  ((n, const_0), Empty))
+            fns in
+     let (xs', frees) = FOLDR (λ(x,l) (nts,frees). x::nts, mk_Union l frees)
+                              ([], Shift m l2)
+                              xls
+     in
+       ([Letrec loc vs_opt xs' (HD c2)], frees)) ∧
   (remove [Handle x1 x2] =
      let (c1,l1) = remove [x1] in
      let (c2,l2) = remove [x2] in
@@ -72,7 +134,9 @@ val remove_def = tDefine "remove" `
      let (c1,l1) = remove xs in
        ([Call dest c1],l1))`
  (WF_REL_TAC `measure exp3_size`
-  \\ REPEAT STRIP_TAC \\ IMP_RES_TAC exp1_size_lemma \\ DECIDE_TAC);
+  \\ REPEAT STRIP_TAC \\ IMP_RES_TAC exp1_size_lemma \\ simp[] >>
+  Induct_on `xs` >> rpt strip_tac >> lfs[exp_size_def] >> res_tac >>
+  simp[exp_size_def]);
 
 val remove_ind = theorem "remove_ind";
 
